add PID

theories/opsem/basic.v
@@ -101,11 +101,28 @@ Proof.
   rewrite decode_encode;done.
 Defined.
 
-Definition Word: Type := nat.
+Definition WordNum : Z :=Z.pow 2 64.
+
+Inductive Word: Type :=
+| W (z : Z) (fin: Z.leb z WordNum = true) (pos: Z.leb 0 z = true).
+
 
 Definition GenReg := gmap GenRegName Word.
 Definition SysReg := gmap SysRegName Word.
 
+Definition GenRegLocate (reg : GenReg) (r : GenRegName) : Word.
+Proof.
+  destruct (reg !! r).
+  - exact w.
+  - exact (W WordNum eq_refl eq_refl).
+Defined.
+
+Definition SysRegLocate (reg : SysReg) (r : SysRegName) : Word.
+Proof.
+  destruct (reg !! r).
+  - exact w.
+  - exact (W WordNum eq_refl eq_refl).
+Defined.
 
 (*Instruction*)
 
@@ -128,12 +145,279 @@ Inductive instr: Type :=
 (* Encoding *)
 
 Class InstrEncoding := {
-  decodeInstr : Z → instr;
-  encodeInstr : instr → Z;
+  decodeInstr : Word → instr;
+  encodeInstr : instr → Word;
 
   decode_encode_instr_inv :
     forall (i: instr), decodeInstr (encodeInstr i) = i;
 }.
 
 
-(*TODO: Memory *)
+(*Memory *)
+
+Definition MemNum : Z := Z.pow 2 48.
+
+Inductive Addr: Type :=
+| A (z : Z) (fin: Z.leb z MemNum = true) (pos: Z.leb 0 z = true).
+
+Definition z_of (a: Addr): Z :=
+  match a with
+  | A z _ _ => z
+  end.
+
+Coercion z_of: Addr >-> Z.
+
+Lemma z_of_eq a1 a2 :
+  z_of a1 = z_of a2 ->
+  a1 = a2.
+Proof.
+  destruct a1, a2; cbn. intros ->.
+  repeat f_equal; apply eq_proofs_unicity; decide equality.
+Qed.
+
+Lemma eq_z_of a1 a2 :
+  a1 = a2 ->
+  z_of a1 = z_of a2.
+Proof. destruct a1; destruct a2. congruence. Qed.
+
+Global Instance addr_eq_dec: EqDecision Addr.
+Proof.
+intros x y. destruct x,y. destruct (Z_eq_dec z z0).
+- left. subst z0. eapply z_of_eq; eauto.
+- right. inversion 1. simplify_eq.
+Defined.
+
+Definition z_to_addr (z : Z) : option Addr.
+Proof.
+  destruct (Z_le_dec z MemNum),(Z_le_dec 0 z).
+  - apply (Z.leb_le z MemNum) in l.
+    apply (Z.leb_le 0 z) in l0.
+    exact (Some (A z l l0)).
+  - exact None.
+  - exact None.
+  - exact None.
+Defined.
+
+Global Instance addr_countable : Countable Addr.
+Proof.
+  refine {| encode r := encode (z_of r) ;
+            decode n := match (decode n) with
+                        | Some z => z_to_addr z
+                        | None => None
+                        end ;
+            decode_encode := _ |}.
+  intro r. destruct r; auto.
+  rewrite decode_encode.
+  unfold z_to_addr. simpl.
+  destruct (Z_le_dec z MemNum),(Z_le_dec 0 z).
+  - repeat f_equal; apply eq_proofs_unicity; decide equality.
+  - exfalso. by apply (Z.leb_le 0 z) in pos.
+  - exfalso. by apply (Z.leb_le z MemNum) in fin.
+  - exfalso. by apply (Z.leb_le z MemNum) in fin.
+Defined.
+
+Definition Mem := gmap Addr Word.
+
+
+Definition MemLocate (mem : Mem) (a : Addr): Word.
+Proof.
+  destruct (mem !! a).
+  - exact w.
+  - exact (W WordNum eq_refl eq_refl).
+Defined.
+
+(*PID*)
+
+Definition PageBitSize : Z := 12.
+
+Definition PIDNum :Z := Z.shiftr MemNum PageBitSize.
+
+Inductive PID :Type :=
+  | P (z:Z) (fin: Z.leb z PIDNum = true) (pos: Z.leb 0 z = true).
+
+(*helper lemmas for pid_of*)
+Lemma iter_div2_zero:forall (s:positive), (0=(Pos.iter Z.div2 0 s))%Z.
+Proof.
+  intro.
+  induction s as [s|s|];simpl.
+  do 2 rewrite <-IHs;done.
+do 2  rewrite <-IHs;done.
+  done.
+Qed.
+
+Lemma iter_div2_noneg:forall (m s:positive), (0≤(Pos.iter Z.div2 (Z.pos m) s))%Z.
+Proof.
+  intros.
+  generalize dependent m.
+  induction s as [s|s|];simpl.
+  - intro.
+    rewrite Z.div2_nonneg.
+    destruct (Pos.iter Z.div2 (Z.pos m) s)%Z eqn:Heqn.
+    rewrite <-(iter_div2_zero s);done.
+    apply (IHs p).
+    assert (0 ≤Z.neg p)%Z.
+    { rewrite <-Heqn. apply (IHs m).}
+    contradiction.
+  - intro.
+    destruct (Pos.iter Z.div2 (Z.pos m) s)%Z eqn:Heqn.
+    rewrite <-(iter_div2_zero s);done.
+    apply (IHs p).
+    assert (0 ≤Z.neg p)%Z.
+    { rewrite <-Heqn. apply (IHs m).}
+    contradiction.
+  - intro.
+    destruct m;simpl;done.
+Qed.
+
+Lemma Zpos_le: forall (m n:positive), (m ≤ n)%positive <-> ((Z.pos m)≤(Z.pos n))%Z.
+Proof.
+  intros.
+  split.
+  - intro.
+    done.
+  - intro.
+    done.
+Qed.
+
+Lemma iter_div2_mono:forall (m n s:positive), (0 ≤ Z.pos s)%Z -> (m≤n)%positive
+        → (Pos.iter Z.div2 (Z.pos m) s ≤ Pos.iter Z.div2 (Z.pos n) s)%Z.
+Proof.
+  intros.
+  generalize dependent m.
+  generalize dependent n.
+  induction s as [s | s|];simpl.
+  - intros.
+    do 2 rewrite Zdiv2_div.
+    apply Z_div_le.
+    done.
+    destruct (Pos.iter Z.div2 (Z.pos m) s)%Z eqn:Heqm.
+    + rewrite <-(iter_div2_zero s).
+      destruct (Pos.iter Z.div2 (Z.pos n) s)%Z eqn:Heqn.
+      * rewrite <-(iter_div2_zero s);done.
+      * apply iter_div2_noneg.
+      * assert (0 ≤Z.neg p)%Z.
+        { rewrite <-Heqn. apply iter_div2_noneg.}
+        contradiction.
+    + destruct (Pos.iter Z.div2 (Z.pos n) s)%Z eqn:Heqn.
+      * rewrite <-(iter_div2_zero s).
+        destruct (Pos.iter Z.div2 (Z.pos p) s)%Z eqn:Heqp.
+        done.
+        exfalso.
+        assert (Z.pos p ≤ 0)%Z.
+        { rewrite <-Heqn, <-Heqm. apply (IHs). done. done. }
+        contradiction.
+        done.
+      * apply IHs.
+        done.
+        rewrite Zpos_le.
+        rewrite <-Heqm,<-Heqn.
+        apply IHs.
+        done.
+        done.
+      * exfalso.
+        assert (Z.pos p ≤ Z.neg p0)%Z.
+        { rewrite <-Heqn, <-Heqm. apply (IHs). done. done. }
+        contradiction.
+    + assert (0 ≤Z.neg p)%Z.
+        { rewrite <-Heqm. apply iter_div2_noneg.}
+        contradiction.
+  - intros.
+    destruct (Pos.iter Z.div2 (Z.pos m) s)%Z eqn:Heqm.
+    + rewrite <-(iter_div2_zero s).
+      destruct (Pos.iter Z.div2 (Z.pos n) s)%Z eqn:Heqn.
+      * rewrite <-(iter_div2_zero s);done.
+      * apply iter_div2_noneg.
+      * assert (0 ≤Z.neg p)%Z.
+        { rewrite <-Heqn. apply iter_div2_noneg.}
+        contradiction.
+    + destruct (Pos.iter Z.div2 (Z.pos n) s)%Z eqn:Heqn.
+      * rewrite <-(iter_div2_zero s).
+        destruct (Pos.iter Z.div2 (Z.pos p) s)%Z eqn:Heqp.
+        done.
+        exfalso.
+        assert (Z.pos p ≤ 0)%Z.
+        { rewrite <-Heqn, <-Heqm. apply (IHs). done. done. }
+        contradiction.
+        done.
+      * apply IHs.
+        done.
+        rewrite Zpos_le.
+        rewrite <-Heqm,<-Heqn.
+        apply IHs.
+        done.
+        done.
+      * exfalso.
+        assert (Z.pos p ≤ Z.neg p0)%Z.
+        { rewrite <-Heqn, <-Heqm. apply (IHs). done. done. }
+        contradiction.
+    + assert (0 ≤Z.neg p)%Z.
+        { rewrite <-Heqm. apply iter_div2_noneg.}
+        contradiction.
+  - intros.
+    destruct m,n;try done.
+    + simpl.
+      rewrite <-Zpos_le.
+      lia.
+    + simpl.
+      rewrite <-Zpos_le.
+      lia.
+Qed.
+
+Lemma shiftr_le: forall (m n s: Z), (0≤m)%Z -> (0≤n)%Z -> (0≤s)%Z-> (m≤n)%Z -> ((m≫s) ≤ (n ≫s))%Z.
+Proof.
+  intros.
+  destruct m ,n; try (rewrite (Z.shiftr_0_l _));auto;try contradiction.
+  - rewrite (Z.shiftr_nonneg _ _). done.
+  - destruct s.
+    + rewrite (Z.shiftr_0_r _).
+      rewrite (Z.shiftr_0_r _).
+      done.
+    + unfold Z.shiftr.
+      unfold Z.shiftl.
+      simpl.
+      apply iter_div2_mono.
+      done.
+      rewrite Zpos_le.
+      done.
+    + unfold Z.shiftr.
+      unfold Z.shiftl.
+      simpl.
+      done.
+Defined.
+
+Definition pid_of (a : Addr) : PID.
+Proof.
+  destruct a.
+  assert(z ≫ PageBitSize ≤ PIDNum)%Z.
+  { unfold PIDNum.
+    apply (Z.leb_le z MemNum) in fin.
+    apply (Z.leb_le 0 z) in pos.
+    apply shiftr_le;done.
+  }
+  apply (Z.leb_le (z≫ PageBitSize) PIDNum) in H.
+    apply (Z.leb_le 0 z) in pos.
+    assert (0≤ (z ≫ PageBitSize))%Z.
+    { apply Z.shiftr_nonneg.  done. }
+   apply (Z.leb_le 0 (z≫ PageBitSize)) in H0.
+    exact (P (z≫ PageBitSize)%Z H H0).
+Defined.
+
+
+(*VMID*)
+
+Definition VMID :Type := nat.
+
+
+(*TODO: MailBox*)
+
+
+
+(*TODO: State*)
+
+
+
+(*TODO: ShareState*)
+
+
+
+(*TODO: ExecConf*)
